Update

Tealeaves/Backends/Named/NamedTraditional.v
@@ -3,9 +3,14 @@ From Tealeaves Require Import
   Classes.Kleisli.DecoratedTraversableMonadPoly
   Functors.List_Telescoping_General
   Backends.Named.Names
-  Backends.Named.Named
+  Backends.Named.Common
+  Backends.Named.Named (FV)
   Functors.Constant
   Functors.Subset.
+
+Export Backends.Named.Names.
+Export Backends.Named.Common.
+Export Backends.Named.Named (FV).
 
 Import Subset.Notations.
 Import Monoid.Notations.
@@ -36,7 +41,7 @@ Ltac step_set_test :=
       progress (repeat rewrite Hf)
   end.
 
-Section alt.
+Section ops.
 
   Context
     {T: Type -> Type -> Type}
@@ -47,339 +52,104 @@ Section alt.
 
   Section rename_local.
 
-    Context (conflicts: list name). (* Top level conflicts, intuitively FV t \cup FV u *)
-
     (* X is the var being substituted, fv_u is FV u *)
-    Context (x: name) (fv_u: list name) (u: T name name).
+    Context
+      (x: name)
+      (u: T name name).
 
+    Context
+      (conflicts: list name)  (* Top level conflicts, intuitively FV t \cup FV u *)
+      (fv_u: list name).  (* Intuitively FV u *)
 
-    (* Given a substitution of x by u, encode the logic of what happens at <<current>> if <<history>> is the set of names
-       given to the binders so far *)
-    Definition rename_binder_local_history:
-      list name * name -> name :=
-      fun '(history, b) =>
-        if x == b
-        then b
-        else if SmartAtom.name_inb b (fv_u)
-             then fresh (conflicts ++ history ++ [b])
-             else if SmartAtom.name_inb b (conflicts ++ history)
-                  then fresh (conflicts ++ history ++ [b])
-                  else b.
+    Definition rename_binder_one (hist: list name) (b: name) :=
+      if b == x
+      then b
+      else if SmartAtom.name_inb b (fv_u)
+           then fresh ([x] ++ conflicts ++ hist ++ [b])
+           else if SmartAtom.name_inb b (hist)
+                then fresh ([x] ++ conflicts ++ hist ++ [b])
+                else b.
 
-    Definition ctx_to_history: list name -> list name :=
-      fold_with_history rename_binder_local_history.
+    Fixpoint rename_binder_from_ctx_rec
+      (ctx: list name)
+      (hist: list name) (b: name): name :=
+      match ctx with
+      | nil =>
+          rename_binder_one hist b
 
-    Lemma rename_binder_local_history_rw1 {hist b}:
-      b = x ->
-      rename_binder_local_history (hist, b) = b.
+      | cons y rest =>
+          if y == x
+          then b
+          else let z := rename_binder_one hist y in
+               rename_binder_from_ctx_rec rest (hist ++ [z]) b
+      end.
+
+    Lemma rename_binder_from_ctx_rec_rw_nil: forall hist b,
+        rename_binder_from_ctx_rec nil hist b =
+          rename_binder_one hist b.
+    Proof.
+      intros. reflexivity.
+    Qed.
+
+    Lemma rename_binder_from_ctx_rec_rw_cons_neq: forall (y: name) (ctx: list name) hist b,
+        y <> x ->
+        rename_binder_from_ctx_rec (y :: ctx) hist b =
+          rename_binder_from_ctx_rec ctx (hist ++ [rename_binder_one hist y]) b.
     Proof.
       intros.
-      unfold rename_binder_local_history.
-      destruct_eq_args x b.
+      cbn.
+      destruct_eq_args y x.
     Qed.
 
-    Lemma rename_binder_local_history_rw2 {hist b}:
-      b <> x ->
-      (b ∈ fv_u) ->
-      rename_binder_local_history (hist, b) = fresh (conflicts ++ hist ++ [b]).
-    Proof.
-      introv BneqX BinFVu.
-      unfold rename_binder_local_history.
-      destruct_eq_args x b.
-      rewrite <- SmartAtom.name_inb_iff in BinFVu.
-      rewrite BinFVu.
-      reflexivity.
-    Qed.
 
-    Lemma rename_binder_local_history_rw2' {b}:
-      b <> x ->
-      b ∈ fv_u ->
-      rename_binder_local_history (nil, b) = fresh (conflicts ++ [b]).
+    Lemma rename_binder_from_ctx_rec_rw_cons_eq: forall (y: name) (ctx: list name) hist b,
+        y = x ->
+        rename_binder_from_ctx_rec (y :: ctx) hist b = b.
     Proof.
       intros.
-      rewrite rename_binder_local_history_rw2; auto.
+      cbn.
+      destruct_eq_args y x.
     Qed.
 
 
-    Lemma rename_binder_local_history_rw3 {hist b}:
-      b <> x ->
-      ~ (b ∈ fv_u) ->
-      (b ∈ (conflicts ++ hist)) ->
-      rename_binder_local_history (hist, b) = fresh (conflicts ++ hist ++ [b]).
-    Proof.
-      introv BneqX BinFVu BninHist.
-      unfold rename_binder_local_history.
-      destruct_eq_args x b.
-      rewrite <- SmartAtom.name_inb_iff_false in BinFVu.
-      rewrite BinFVu.
-      step_set_test.
-      reflexivity.
-    Qed.
-
-
-    Lemma rename_binder_local_history_rw4 {hist b}:
-      b <> x ->
-      ~ (b ∈ fv_u) ->
-      ~ (b ∈ (conflicts ++ hist)) ->
-      rename_binder_local_history (hist, b) = b.
-    Proof.
-      introv BneqX BinFVu BninHist.
-      unfold rename_binder_local_history.
-      destruct_eq_args x b.
-      rewrite <- SmartAtom.name_inb_iff_false in BinFVu.
-      rewrite BinFVu.
-      step_set_test.
-      reflexivity.
-    Qed.
-
-
-    Lemma ctx_to_history_nil: ctx_to_history [] = [].
-    Proof.
-      intros.
-      reflexivity.
-    Qed.
-
-    Lemma ctx_to_history_cons1 {nm l}:
-      x = nm ->
-      ctx_to_history (nm :: l) =
-        nm :: fold_with_history (rename_binder_local_history ⦿ [nm]) l.
-    Proof.
-      intros.
-      unfold ctx_to_history.
-      rewrite fold_with_history_cons.
-      rewrite rename_binder_local_history_rw1; auto.
-    Qed.
-
-
-    Lemma ctx_to_history_cons_cons2 {nm l}:
-      x <> nm ->
-      (nm ∈ fv_u) ->
-      ctx_to_history (nm :: l) =
-        fresh (conflicts ++ [nm]) :: fold_with_history (rename_binder_local_history ⦿ [fresh (conflicts ++ [nm])]) l.
-    Proof.
-      intros.
-      unfold ctx_to_history.
-      rewrite fold_with_history_cons.
-      rewrite rename_binder_local_history_rw2'; auto.
-    Qed.
-
-    Lemma ctx_to_history_cons_rw3 {nm l}:
-      x <> nm ->
-      ~ (nm ∈ fv_u) ->
-      nm ∈ (conflicts) ->
-      ctx_to_history (nm :: l) =
-        fresh (conflicts ++ [nm]) :: fold_with_history (rename_binder_local_history ⦿ [fresh (conflicts ++ [nm])]) l.
-    Proof.
-      intros.
-      unfold ctx_to_history.
-      rewrite fold_with_history_cons.
-      rewrite rename_binder_local_history_rw3; auto.
-      rewrite List.app_nil_r.
-      assumption.
-    Qed.
-
-    Lemma ctx_to_history_cons_rw4 {nm l}:
-      x <> nm ->
-      ~ (nm ∈ fv_u) ->
-      ~ nm ∈ (conflicts) ->
-      ctx_to_history (nm :: l) =
-        nm :: fold_with_history (rename_binder_local_history ⦿ [nm]) l.
-    Proof.
-      intros.
-      unfold ctx_to_history.
-      rewrite fold_with_history_cons.
-      rewrite rename_binder_local_history_rw4; auto.
-      rewrite List.app_nil_r.
-      assumption.
-    Qed.
-
-    Lemma ctx_to_history_app: forall l1 l2,
-        ctx_to_history (l1 ++ l2) =
-          ctx_to_history l1 ++
-            (fold_with_history (rename_binder_local_history ⦿ fold_with_history rename_binder_local_history l1) l2).
-    Proof.
-      intros.
-      unfold ctx_to_history.
-      rewrite fold_with_history_app.
-      reflexivity.
-    Qed.
-
-
-    (*
-
-    (* Name a binder to something else during substitution *)
-    Definition rename_binder_local:
+    Definition rename_binder_from_ctx:
       list name * name -> name :=
       fun '(ctx, b) =>
-        if SmartAtom.name_inb x ctx (* Halt substitution early, we didn't recurse where x appears in ctx *)
-        then b
-        else if x == b (* Else check if halt now *)
-             then b (* This binder is the name of the free variable we're substituting, halt and leave binder alone *)
-             else if SmartAtom.name_inb b fv_u (* Else check if need to rename *)
-                  then (rename_binder_local_history (ctx_to_history ctx, b))
-                  else b.
+        rename_binder_from_ctx_rec ctx [] b.
 
-    (* This binder is under an abstraction of the substituted variable, do nothing (subst halted earlier) *)
-    Lemma rename_binder_local_rw1: forall ctx b,
-        x ∈ ctx ->
-        rename_binder_local (ctx, b) = b.
-    Proof.
-      intros.
-      unfold rename_binder_local.
-      step_set_test.
-      reflexivity.
-    Qed.
+    Definition context_to_renamed:
+      list name -> list name :=
+      fold_with_history rename_binder_from_ctx.
 
-    (* This binder is equal to the variable begin substituted (subst is halting now) *)
-    Lemma rename_binder_local_rw2: forall ctx b,
-        ~ (x ∈ ctx) ->
-        x = b ->
-        rename_binder_local (ctx, b) = b.
-    Proof.
-      intros.
-      unfold rename_binder_local.
-      destruct_eq_args x b.
-      now step_set_test.
-    Qed.
-
-    (* This binder conflicts with the free variables of u, rename after computing its history from its context *)
-    Lemma rename_binder_local_rw3: forall ctx b,
-        ~ (x ∈ ctx) ->
-        x <> b ->
-        b ∈ fv_u ->
-        rename_binder_local (ctx, b) = (rename_binder_local_history (ctx_to_history ctx, b)).
-    Proof.
-      intros.
-      unfold rename_binder_local.
-      step_set_test.
-      destruct_eq_args x b.
-      step_set_test.
-      reflexivity.
-    Qed.
-
-    (* This is a bound variable that doesn't cause any conflicts, do nothing *)
-    Lemma rename_binder_local_rw4: forall ctx b,
-        ~ (x ∈ ctx) ->
-        x <> b ->
-        ~ (b ∈ fv_u) ->
-        rename_binder_local (ctx, b) = b.
-    Proof.
-      intros.
-      subst.
-      unfold rename_binder_local.
-      destruct (SmartAtom.name_inb x ctx); auto.
-      destruct_eq_args x b.
-      step_set_test.
-      reflexivity.
-    Qed.
-
-    Corollary rename_binder_local_rw5: forall ctx b,
-        ~ (b ∈ fv_u) ->
-        rename_binder_local (ctx, b) = b.
-    Proof.
-      intros.
-      unfold rename_binder_local.
-      destruct (SmartAtom.name_inb x ctx).
-      - reflexivity.
-      - destruct_eq_args x b.
-        step_set_test.
-        reflexivity.
-    Qed.
-
-    Lemma rename_binder_local_spec:
-      forall '(ctx, b),
-        rename_binder_local (ctx, b) = rename_binder_local_history (ctx_to_history ctx, b).
-    Proof.
-      intros [ctx b].
-      destruct (destruct_in x ctx).
-      rewrite rename_binder_local_rw1.
-      rewrite rename_binder_local_history_rw1.
-
-      step_set_test.
-      rewrite rename_binder_local_history_rw2.
-
-     *)
-
- Definition rename_binder_local:
-      list name * name -> name :=
-   fun '(ctx, b) =>
-     rename_binder_local_history (ctx_to_history ctx, b).
-
- Definition subst_local:
-   list name * name -> T name name :=
-   fun '(ctx, v) =>
-     if SmartAtom.name_inb x ctx (* Halt substitution early *)
-     then ret (T := T name) v
-     else
-       match (get_binding ctx v) with
-       | Unbound _ =>
-           if v == x
-           then u
-           else ret (T := T name) v
-       | Bound prefix _ _ =>
-           ret (T := T name) (rename_binder_local (prefix, v))
-       end.
-
-
- (* This variable is under an abstraction of the substituted variable, do nothing (subst halted earlier) *)
- Lemma subst_local_rw1: forall ctx v,
-     x ∈ ctx ->
-     subst_local (ctx, v) = ret v.
- Proof.
-   intros.
-   unfold subst_local.
-   step_set_test.
-   reflexivity.
- Qed.
-
- (* This variable is equal to the variable begin substituted, replace it *)
- Lemma subst_local_rw2: forall ctx v,
-     ~ (x ∈ ctx) ->
-     x = v ->
-     subst_local (ctx, v) = u.
- Proof.
-   intros.
-   unfold subst_local.
-   destruct_eq_args x v.
-   step_set_test.
-   rewrite get_binding1; auto.
- Qed.
-
- Lemma hmmm:forall ctx v,
-     ~ v ∈ ctx ->
-     v = (rename_binder_local_history (ctx_to_history ctx, v)).
- Proof.
-   intros.
- Abort.
-
-
- (* This is a bound variable that  conflicts with the free variables of u,
-       rename it to match its binder *)
- Lemma subst_local_rw3: forall pre post ctx v,
-     ~ (x ∈ ctx) ->
-     x <> v ->
-     get_binding ctx v = Bound pre v post ->
-     subst_local (ctx, v) = ret (rename_binder_local_history (ctx_to_history pre, v)).
- Proof.
-   intros.
-   unfold subst_local.
-   step_set_test.
-   rewrite H3.
-   unfold rename_binder_local.
-   reflexivity.
- Qed.
-
- Definition subst_top
-   (t: T name name): T name name :=
-   substitute (G := fun A => A) (U := T)
-     rename_binder_local
-     subst_local t.
+    Definition subst_from_ctx:
+      list name * name -> T name name :=
+      fun '(ctx, v) =>
+        match get_binding ctx v with
+        | Unbound _ =>
+            (* v is a free variable *)
+            if v == x
+            then u
+            else ret v
+        | Bound prefix _ post =>
+            (* v is a bound variable, give it the name of whatever it was bound to *)
+            ret (rename_binder_from_ctx (prefix, v))
+        end.
 
   End rename_local.
+
+
+  Definition subst_top
+    (x: name) (u: T name name)
+    (conflicts fv_u: list name)
+   (t: T name name): T name name :=
+   substitute (G := fun A => A) (U := T)
+     (rename_binder_from_ctx x conflicts fv_u)
+     (subst_from_ctx x u conflicts fv_u) t.
 
   Definition subst
     (x: name) (u: T name name)
     (t: T name name): T name name :=
-    subst_top (FV T t ++ FV T u) x (FV T u) u t.
 
-End alt.
+    subst_top x u (FV T t ++ FV T u) (FV T u) t.
+
+End ops.
