Tealeaves/Examples/LambdaNominal/Equivalence.v
@@ -14,6 +14,7 @@ From Tealeaves Require Export
 Import DecoratedTraversableMonadPoly.DerivedOperations.
 Import Kleisli.DecoratedTraversableMonadPoly.DerivedOperations.
 Import Kleisli.DecoratedTraversableMonadPoly.
+Import ContainerFunctor.Notations.
 
 #[local] Generalizable Variables G.
 
@@ -27,10 +28,10 @@ Section rw.
     `{Applicative G}
     {g: list B1 * B1 -> G B2}
     {f: list B1 * V1 -> G (term B2 V2)}.
-  Lemma sub_term_spec: forall v,
-      substitute (Substitute := Binddt_Categorical term) g f (tvar v) =
-        substitute (Substitute := Substitute_lambda_term) g f (tvar v).
-  Proof.
+    Lemma sub_term_spec: forall v,
+    substitute (Substitute := Binddt_Categorical term) g f (tvar v) =
+    substitute (Substitute := Substitute_lambda_term) g f (tvar v).
+    Proof.
     intros.
     unfold substitute.
     unfold Binddt_Categorical.
@@ -42,10 +43,9 @@ Section rw.
     rewrite mon_join_ret.
     rewrite fun_map_id.
     reflexivity.
-  Qed.
+    Qed.
 
 End rw.
-
 
 Lemma FV_loc_preincr: forall (bs: list name) (t: term name name),
     substitute (B2 := False) (A2 := False)
@@ -90,7 +90,7 @@ Proof.
     admit.
 Admitted.
 
-Lemma FV_fvL : forall (t: term name name),
+Lemma FV_fvL: forall (t: term name name),
     FV term t = fvL t.
 Proof.
   intros t.
@@ -104,65 +104,26 @@ Proof.
   admit.
 Admitted.
 
-(*
-Section rw.
-
-  Context (x: name) (u: term name name).
-
-  Lemma subst_term_rw1: forall (v: name),
-      Named.subst term x u (tvar v) =
-        if (v == x) then u else (tvar v).
-  Proof.
-    reflexivity.
-  Qed.
-  Lemma subst_conflicts_rw1: forall top (v: name),
-      subst_conflicts term top x u (tvar v) =
-        if (v == x) then u else (tvar v).
-  Proof.
-    reflexivity.
-  Qed.
-
-  Lemma subst_conflicts_rw2: forall (top: list name) (b: name) (t: term name name),
-      subst_conflicts term top x u (lam b t) =
-        lam (rename_binder_local top ([], b))
-          (DecoratedTraversableMonadPoly.substitute (G := fun A => A)
-             (rename_binder_local top ⦿ [b])
-             (subst_local top x u ⦿ [b]) t).
-  Proof.
-    intros.
-    reflexivity.
-  Qed.
-
-  Lemma subst_conflicts_rw3: forall (top: list name) (t1 t2: term name name),
-      subst_conflicts term top x u (tap t1 t2) =
-        tap (subst_conflicts term top x u t1) (subst_conflicts term top x u t2).
-  Proof.
-    reflexivity.
-  Qed.
-End rw.
-*)
-
-
 Section rw.
 
   Context
-    (top: list name)
-    (x: name) (fv_u: list name) (u: term name name).
+    (conflicts: list name)
+    (fv_u: list name)
+    (x: name) (u: term name name).
 
   Lemma subst_top_rw1: forall (v: name),
-      subst_top top x fv_u u (tvar v) =
+      subst_top x u conflicts fv_u (tvar v) =
         if (v == x) then u else (tvar v).
   Proof.
     reflexivity.
   Qed.
 
-
   Lemma subst_top_rw2: forall (b: name) (t: term name name),
-      subst_top top x (fv_u) u (lam b t) =
-        lam (rename_binder_local top x fv_u ([], b))
+      subst_top x u  conflicts (fv_u) (lam b t) =
+        lam (rename_binder_from_ctx x conflicts fv_u ([], b))
           (substitute (G := fun A => A)
-             (rename_binder_local top x fv_u ⦿ [b])
-             (subst_local top x fv_u u ⦿ [b]) t).
+             (rename_binder_from_ctx x conflicts fv_u ⦿ [b])
+             (subst_from_ctx x u conflicts fv_u ⦿ [b]) t).
   Proof.
     intros.
     unfold subst_top.
@@ -172,235 +133,350 @@ Section rw.
   Qed.
 
   Lemma subst_top_rw3: forall (top: list name) (t1 t2: term name name),
-      subst_top top x fv_u u (tap t1 t2) =
-        tap (subst_top top x fv_u u t1) (subst_top top x fv_u u t2).
+      subst_top x u conflicts fv_u (tap t1 t2) =
+        tap (subst_top x u conflicts fv_u t1) (subst_top x u conflicts fv_u t2).
   Proof.
     reflexivity.
   Qed.
 
 End rw.
 
-
-
-
-Import ContainerFunctor.Notations.
-
-(*
-Lemma rename_binder_kill2: forall top x fv_u,
-    rename_binder_local top x fv_u ([], x) = x.
-Proof.
-  intros.
-  cbn.
-  destruct_eq_args x x.
-Qed.
-
-
-Lemma subst_local_kill: forall top x fv_u u l ctx v,
-    x ∈ l ->
-    (subst_local top x fv_u u ⦿ l) (ctx, v) = tvar v.
-Proof.
-  intros.
-  change (subst_local top x fv_u u (l ++ ctx, v) = tvar v).
-  unfold subst_local.
-  remember (SmartAtom.name_inb x (l ++ ctx)).
-  destruct b.
-  + reflexivity.
-  + false.
-    symmetry in Heqb.
-    rewrite SmartAtom.name_inb_iff_false in Heqb.
-    rewrite element_of_list_app in Heqb.
-    intuition.
-Qed.
-
-
-Lemma kill:
-  forall (top fv_u: list name) (any: list name) (x: name) (t u: term name name),
-    x ∈ any ->
-    substitute (T := term) (G := fun A => A)
-      (rename_binder_local top x fv_u ⦿ any)
-      (subst_local top x fv_u u ⦿ any) t = t.
-Proof.
-  intros.
-  change t with (id t) at 2.
-  rewrite <- (kdtmp_substitute1 (T := term) (B := name) (A := name)).
-  fequal.
-  - ext (ctx, v).
-    now apply rename_binder_kill.
-  - ext (ctx, v).
-    now apply subst_local_kill.
-Qed.
-
-Lemma inb_iff: forall (l: list name) (x: name),
-    SmartAtom.name_inb x l = false <-> (~ x ∈ l).
-Proof.
-  induction l.
-  - cbv. intuition.
-  - intros. cbn.
-    destruct_eq_args x a.
-    + cbn. firstorder. inversion H.
-    + cbn. rewrite IHl. firstorder.
-Qed.
-
-Lemma inb_iff2: forall (l: list name) (x: name),
-    SmartAtom.name_inb x l = true <-> (x ∈ l).
-Proof.
-  induction l.
-  - cbv. intuition.
-  - intros. cbn.
-    destruct_eq_args x a.
-    + cbn. firstorder.
-    + cbn. rewrite IHl. firstorder.
-Qed.
-
-Lemma x1: forall top x l ctx b,
-    ~ (b ∈ l) ->
-    (rename_binder_local top x l (ctx, b)) = b.
-Proof.
-  intros. cbn.
-  destruct (SmartAtom.name_inb x ctx).
-  - reflexivity.
-  - destruct_eq_args b x.
-    rewrite <- inb_iff in H.
-    rewrite H.
-    reflexivity.
-Qed.
-
-Lemma rename_binder_preincr1: forall top x l b,
-    b = x ->
-    ~ (b ∈ l) ->
-    rename_binder_local top x l ⦿ [b] =
+Lemma lemma1: forall
+    (conflicts: list name) (fv_u: list name) (x:name),
+    (rename_binder_from_ctx x conflicts fv_u) ⦿ [x] =
       extract.
 Proof.
   intros.
-  ext (ctx, v).
-  unfold preincr, compose, incr.
-  unfold_ops @Monoid_op_list.
-  unfold rename_binder_local.
-  subst.
-  assert (SmartAtom.name_inb x ([x] ++ ctx) = true).
-  { rewrite SmartAtom.name_inb_iff.
-    firstorder. }
-  rewrite H.
-  reflexivity.
-Qed.
- *)
-
-
-
-
-(*
-Lemma needed_easier:forall (top:list name) (x:name) (l:list name) (b:name) (ctx:list name) v,
-    b <> x ->
-    ~ (b ∈ l) ->
-    v ∈ l ->
-  (rename_binder_local_history top x l ⦿ [b]) (ctx, v) =
-    (rename_binder_local_history (top ++ [b]) x l) (ctx, v).
-Proof.
-  intros.
-  unfold preincr, compose, incr.
-  change (?a ● ?g) with (a ++ g).
-  destruct ctx.
-  - rewrite List.app_nil_r.
-    unfold rename_binder_local_history.
-    destruct_eq_args x v.
-    rewrite <- SmartAtom.name_inb_iff in H1.
-    rewrite H1.
-    rewrite List.app_nil_l.
-    rewrite List.app_assoc.
-    reflexivity.
-  - unfold rename_binder_local_history.
-    destruct_eq_args x v.
-    rewrite <- SmartAtom.name_inb_iff in H1.
-    rewrite H1.
-    change (?x :: ctx) with ([x] ++ ctx).
-    repeat rewrite List.app_assoc.
-    reflexivity.
+  ext (ctx, b).
+  unfold preincr, incr, compose.
+  change ([x] ● ctx) with (x::ctx).
+  unfold rename_binder_from_ctx.
+  rewrite rename_binder_from_ctx_rec_rw_cons_eq; auto.
 Qed.
 
-Lemma needed_harded:forall (top:list name) (x:name) (l:list name) (b:name) (ctx:list name) v,
-    b <> x ->
-    ~ (b ∈ l) ->
-    ~ v ∈ l ->
-  (rename_binder_local_history top x l ⦿ [b]) (ctx, v) =
-    (rename_binder_local_history (top ++ [b]) x l) (ctx, v).
-Proof.
-  intros.
-  unfold preincr, compose, incr.
-  change (?a ● ?g) with (a ++ g).
-  destruct ctx.
-  - rewrite List.app_nil_r.
-    unfold rename_binder_local_history.
-    destruct_eq_args x v.
-    rewrite <- SmartAtom.name_inb_iff_false in H1.
-    rewrite H1.
-    reflexivity.
-  - unfold rename_binder_local_history.
-    destruct_eq_args x v.
-    destruct (SmartAtom.name_inb v l); auto.
-    repeat rewrite List.app_assoc.
-    reflexivity.
-Qed.
-
-Lemma needed_yay:forall (top:list name) (x:name) (l:list name) (b:name) (ctx:list name) v,
-    b <> x ->
-    ~ (b ∈ l) ->
-  (rename_binder_local_history top x l ⦿ [b]) (ctx, v) =
-    (rename_binder_local_history (top ++ [b]) x l) (ctx, v).
-Proof.
-  intros.
-  destruct (destruct_in v l).
-  - apply needed_easier; auto.
-  -  apply needed_harded; auto.
-Qed.
-
-Lemma needed_yayy:forall (top:list name) (x:name) (l:list name) (b:name),
-    b <> x ->
-    ~ (b ∈ l) ->
-  (rename_binder_local_history top x l ⦿ [b]) =
-    (rename_binder_local_history (top ++ [b]) x l).
+Lemma lemma2: forall
+    (conflicts: list name) (fv_u: list name) (x:name) (u: term name name),
+    (subst_from_ctx x u conflicts fv_u) ⦿ [x] =
+      ret ∘ extract.
 Proof.
   intros.
   ext (ctx, v).
-  now apply needed_yay.
+  unfold preincr, incr, compose.
+  change ([x] ● ctx) with (x::ctx).
+  unfold subst_from_ctx.
+  destruct (get_binding_spec (x :: ctx) v) as [[Heq Hnin]| H2].
+  - rewrite Heq.
+    assert (v <> x).
+    rewrite element_of_list_cons in Hnin. tauto.
+    destruct_eq_args v x.
+  - destruct H2 as [pre [post [rest1 [rest2 rest3]]]].
+    rewrite rest1.
+    cbn.
+    destruct pre.
+    + cbn. fequal.
+      assert (x = v).
+      { now inversion rest2. }
+      subst.
+      unfold rename_binder_one.
+      destruct_eq_args v v.
+    +
+      assert (x = n).
+      { now inversion rest2. }
+      subst.
+      change_left (ret ((rename_binder_from_ctx n conflicts fv_u ⦿ [n]) (pre, v))).
+      rewrite lemma1.
+      reflexivity.
 Qed.
 
-Lemma needed_intermediate: forall  top x l b ctx,
 
-    b <> x ->
-    ~ b ∈ l ->
-    fold_with_history (rename_binder_local_history top x l ⦿ [b]) ctx =
-      fold_with_history (rename_binder_local_history (top ++ [b]) x l) ctx.
+Section interpret.
+
+  Context
+    (conflicts: list name)
+  (fv_u: list name) (x: name) (u: term name name).
+
+  Definition interpret_context_to_renamings  (context: list name):
+    term name name -> term name name :=
+    match context with
+    | nil => id
+    | cons b rest =>
+        if b == x
+        then id
+        else if SmartAtom.name_inb x fv_u
+             then let z := (fresh ([x] ++ l ++ [b]): name) in
+                  interpret_context_to_renamings rest ∘ rename b z
+                  else substF conflicts x u
+                  end.
+
+Definition interpret_context (conflicts: list name) (fv_u: list name) (x: name) (u: term name name) (context: list name):
+  term name name -> term name name :=
+  match context with
+  | nil => substF conflicts x u
+  | cons b rest =>
+      if b == x
+      then substF conflicts x u
+      else if SmartAtom.name_inb x fv_u
+           then substF (conflicts ++ context_to_renamed context) x u
+           else substF conflicts x u
+  end.
+
+Lemma equiv_key:
+  forall (conflicts: list name) (x: name) (u: term name name) (context: list name) (t: term name name),
+     substitute (T := term) (G := fun A => A)
+       (rename_binder_from_ctx x conflicts (FV term u) ⦿ context)
+       (subst_from_ctx x u conflicts (FV term u) ⦿ context) t =
+       interpret_context conflicts (FV term u) x u context t.
 Proof.
   intros.
-    induction ctx.
-  - reflexivity.
-  - rewrite fold_with_history_cons.
-    rewrite fold_with_history_cons.
-    fequal.
-    { unfold preincr, compose, incr.
-      change ([b] ● []) with [b].
-      unfold rename_binder_local_history.
-      destruct_eq_args x a.
-      destruct (destruct_in a l).
-      { rewrite <- SmartAtom.name_inb_iff in H1.
-        rewrite H1.
+  induction t.
+  - rewrite sub_term_rw1.
+    unfold preincr, incr, compose.
+    change (@nil name) with (Ƶ:list name).
+    rewrite monoid_id_l.
+    induction context.
+
+
+Theorem woah:
+  forall (conflicts: list name) (x: name) (u: term name name) (b: name) (t: term name name),
+    (~ b ∈ fvL u ->
+     b <> x ->
+     substitute (T := term) (G := fun A => A)
+       (rename_binder_from_ctx x conflicts (FV term u) ⦿ [b])
+       (subst_from_ctx x u conflicts (FV term u) ⦿ [b]) t =
+       substF (conflicts ++ [b]) x u t) /\
+      (b ∈ fvL u ->
+       b <> x ->
+       substitute (T := term) (G := fun A => A)
+         (rename_binder_from_ctx x conflicts (FV term u) ⦿ [b])
+         (subst_from_ctx x u conflicts (FV term u) ⦿ [b]) t =
+         substF (conflicts ++ [fresh ([x] ++ conflicts ++ [b])]) x u (rename b (fresh ([x] ++ conflicts ++ [b])) t)).
+Proof.
+  intros.
+  generalize dependent conflicts.
+  generalize dependent b.
+  induction t.
+  - admit.
+  - (* λ b t *)
+    intros c conflicts.
+    rewrite sub_term_rw2.
+    simplify_applicative_I.
+    unfold ap, mult, Mult_I; unfold_ops @Map_I.
+    split.
+    { introv Hnin Hneq.
+      rewrite substF_rw2.
+      assert (b <> x). admit.
+      destruct_eq_args b x.
+      { rewrite preincr_preincr.
+Abort.
+
+
+Theorem subst_preincr_inFV_spec:
+  forall (conflicts: list name) (x: name) (u: term name name) (b: name) (t: term name name),
+      b ∈ fvL u ->
+      b <> x ->
+      substitute (T := term) (G := fun A => A)
+        (rename_binder_from_ctx x conflicts (FV term u) ⦿ [b])
+        (subst_from_ctx x u conflicts (FV term u) ⦿ [b]) t =
+  substF (conflicts ++ [fresh ([x] ++ conflicts ++ [b])]) x u (rename b (fresh ([x] ++ conflicts ++ [b])) t).
+Proof.
+  introv Hin Hneq.
+  generalize dependent conflicts.
+  generalize dependent b.
+  induction t; intros.
+  - rewrite sub_term_rw1.
+    rewrite rename_rw1.
+    destruct_eq_args v b.
+    + rewrite substF_rw1.
+      unfold preincr, incr, compose.
+      change ([b] ● []) with ([b]).
+      unfold subst_from_ctx.
+      assert (get_binding [b] b = Bound [] b []).
+      { cbn. destruct_eq_args b b. }
+      rewrite H.
+      assert (fresh ([x] ++ conflicts ++ [b]) <> x).
+      { intro contra.
+        assert (~ x ∈ ([x] ++ conflicts ++ [b])).
+        symmetry in contra.
+        rewrite contra at 1.
+        apply SmartAtom.fresh_not_in.
+        rewrite element_of_list_app in H0.
+        rewrite element_of_list_one in H0.
+        tauto.
+      }
+      destruct_eq_args (fresh ([x] ++ conflicts ++ [b])) x.
+      { intuition. }
+      { fequal.
+        unfold rename_binder_from_ctx.
+        unfold rename_binder_from_ctx_rec.
+        unfold rename_binder_one.
+        destruct_eq_args b x.
+        rewrite FV_fvL.
+        step_set_test.
         rewrite List.app_nil_l.
-        rewrite List.app_assoc.
         reflexivity.
       }
-      {rewrite <- SmartAtom.name_inb_iff_false in H1.
-       rewrite H1.
-       reflexivity.
+    +
+      unfold preincr, incr, compose.
+      change ([b] ● []) with ([b]).
+      unfold subst_from_ctx.
+      assert (get_binding [b] v = Unbound [b]).
+      { cbn. destruct_eq_args b v. }
+      rewrite H.
+      destruct_eq_args v x.
+      { rewrite substF_rw1.
+        destruct_eq_args x x.
+      }
+      { rewrite substF_rw1.
+        destruct_eq_args v x.
+      }
+  - rewrite sub_term_rw2.
+    simplify_applicative_I.
+    unfold ap, mult, Mult_I; unfold_ops @Map_I.
+    rewrite rename_rw2_neq.
+
+    rewrite substF_rw2.
+    admit.
+    admit.
+  - rewrite rename_rw3.
+    rewrite substF_rw3.
+    rewrite <- IHt1; auto.
+    rewrite <- IHt2; auto.
+Admitted.
+
+Lemma tvar_helper:
+  forall (conflicts: list name) (x: name) (u: term name name) (b: name) (t: term name name) v,
+    ~ b ∈ fvL u ->
+     b <> x ->
+     subst_from_ctx x u conflicts (FV term u) ([b], v) = (if v == x then u else tvar v).
+Proof.
+  intros.
+  cbn.
+  destruct_eq_args v b.
+  destruct_eq_args b x.
+  cbn.
+  unfold rename_binder_one.
+  destruct_eq_args b x.
+  rewrite FV_fvL.
+  step_set_test.
+  destruct (destruct_in b []).
+  inversion H2.
+  now step_set_test.
+Qed.
+
+
+Theorem subst_preincr_ninFV_spec:
+  forall (conflicts: list name) (x: name) (u: term name name) (b: name) (t: term name name),
+      ~ b ∈ fvL u ->
+      b <> x ->
+    substitute (T := term) (G := fun A => A)
+      (rename_binder_from_ctx x conflicts (FV term u) ⦿ [b])
+      (subst_from_ctx x u conflicts (FV term u) ⦿ [b]) t =
+      substF (conflicts ++ [b]) x u t.
+Proof.
+  introv Hnin Nneq.
+  generalize dependent conflicts.
+  generalize dependent b.
+  induction t; intros.
+  - rewrite sub_term_rw1.
+    rewrite substF_rw1.
+    unfold preincr, incr, compose.
+    change ([b] ● []) with ([b]).
+    rewrite tvar_helper; auto.
+  - rewrite sub_term_rw2.
+    simplify_applicative_I.
+    unfold ap, mult, Mult_I; unfold_ops @Map_I.
+    rewrite substF_rw2.
+
+    destruct_eq_args b x.
+    { fequal.
+      { unfold rename_binder_from_ctx.
+        unfold preincr, incr, compose.
+        change ([b0] ● []) with ([b0]).
+        cbn.
+        destruct_eq_args b0 x.
+        admit.
+      }
+      {
+        specialize (IHt b0 Hnin Nneq).
+        admit.
       }
     }
-    { fequal.
-      rewrite needed_yayy; auto.
+    { destruct (SmartAtom.name_inb b (fvL u)).
+      admit.
+      admit.
     }
+  - cbn.
+    rewrite substF_rw3.
+    rewrite <- IHt1.
+    rewrite <- IHt2.
+    reflexivity.
+Admitted.
+
+Theorem equivalence:
+  forall (conflicts: list name) (x: name) (u: term name name),
+    subst_top x u conflicts (FV term u) =
+      substF conflicts x u.
+Proof.
+  intros. ext t.
+  induction t.
+  - rewrite subst_top_rw1.
+    rewrite substF_rw1.
+    reflexivity.
+  - rewrite subst_top_rw2.
+    rewrite substF_rw2.
+    destruct_eq_args b x.
+    {
+      fequal.
+      { cbn.
+        unfold rename_binder_one.
+        destruct_eq_args x x.
+      }
+      {
+        rewrite lemma1.
+        unfold rename_binder_one.
+        rewrite lemma2.
+        rewrite kdtmp_substitute1.
+        reflexivity.
+      }
+    }
+    { destruct (destruct_in b (fvL u)).
+      { step_set_test.
+        fequal.
+        { unfold rename_binder_from_ctx.
+          rewrite rename_binder_from_ctx_rec_rw_nil.
+          unfold rename_binder_one.
+          destruct_eq_args b x.
+          rewrite FV_fvL.
+          step_set_test.
+          rewrite List.app_nil_l.
+          reflexivity.
+        }
+        {
+          apply subst_preincr_inFV_spec; auto.
+        }
+      }
+      { step_set_test.
+        fequal.
+        { cbn.
+          unfold rename_binder_one.
+          destruct_eq_args b x.
+          rewrite FV_fvL.
+          step_set_test.
+          destruct (destruct_in b []).
+          inversion H2.
+          now step_set_test.
+        }
+        {
+          rewrite subst_preincr_ninFV_spec; auto.
+        }
+      }
+    }
+  - cbn.
+    rewrite substF_rw3.
+    rewrite <- IHt1.
+    rewrite <- IHt2.
+    reflexivity.
 Qed.
-*)
-
-
-
 
 
 Lemma rename_binder_local_history_preincr_spec:
@@ -423,308 +499,3 @@ Proof.
     reflexivity.
 Qed.
 
-Lemma fold_rename_binder_local_history_preincr_spec: forall
-  (conflicts: list name) (x:name) (fv_u: list name) (b:name) (ctx:list name),
-
-    b <> x ->
-    ~ b ∈ fv_u ->
-    fold_with_history (rename_binder_local_history conflicts x fv_u ⦿ [b]) ctx =
-      fold_with_history (rename_binder_local_history (conflicts ++ [b]) x fv_u) ctx.
-Proof.
-  intros.
-  rewrite rename_binder_local_history_preincr_spec; auto.
-Qed.
-
-(*
-Lemma needed:
-  forall (conflicts: list name) (x:name) (fv_u: list name) (b:name) (ctx: list name) (v: name),
-    ~ x ∈ ([b] ++ ctx) ->
-    ~ (x ∈ ctx) ->
-    b <> x ->
-    ~ (b ∈ fv_u) ->
-    v ∈ fv_u ->
-    v <> x ->
-    rename_binder_local conflicts x fv_u ([b] ++ ctx, v) =
-      rename_binder_local (conflicts ++ [b]) x fv_u (ctx, v).
-Proof.
-  intros.
-  unfold rename_binder_local.
-  rewrite ctx_to_history_cons_rw2.
-  rewrite rename_binder_local_history_preincr_spec; auto.
-  rewrite rename_binder_local_history_rw2; auto.
-  rewrite rename_binder_local_history_rw2; auto.
-  change (?x :: ?y) with ([x] ++ y).
-  repeat rewrite <- List.app_assoc.
-  rewrite List.app_nil_r.
-  rewrite List.app_nil_l.
-  reflexivity.
-Qed.
-*)
-
-(*
-Lemma rename_binder_local_preincr: forall
-  (conflicts: list name) (x:name) (fv_u: list name) (b:name),
-    b <> x ->
-    ~ (b ∈ fv_u) ->
-    rename_binder_local conflicts x fv_u ⦿ [b] =
-      rename_binder_local (conflicts ++ [b]) x fv_u.
-Proof.
-  introv BneqX BninFVu.
-  ext (ctx, v).
-  unfold preincr, compose, incr.
-  unfold_ops @Monoid_op_list.
-  destruct (destruct_in x ([b] ++ ctx)) as [Hxin|Hxnin].
-  { (* X is in context *)
-    rewrite rename_binder_local_rw1; auto.
-    rewrite element_of_list_app in Hxin.
-    rewrite element_of_list_one in Hxin.
-    destruct Hxin.
-    + subst. contradiction.
-    + rewrite rename_binder_local_rw1; auto.
-  }
-  { assert (x <> b /\ ~ x ∈ ctx) as Hyp.
-    { rewrite element_of_list_app in Hxnin.
-      rewrite element_of_list_one in Hxnin.
-      firstorder. }
-    destruct Hyp as [Xneqb Xninctx].
-    destruct_eq_args v x.
-    { rewrite rename_binder_local_rw2; auto.
-      rewrite rename_binder_local_rw2; auto.
-    }
-    { destruct (destruct_in v fv_u).
-      { apply needed; auto.
-      }
-      { rewrite rename_binder_local_rw4; auto.
-        rewrite rename_binder_local_rw4; auto.
-      }
-    }
-  }
-Qed.
-*)
-
-
-(*
-Lemma subst_local_kill: forall top x fv_u u l ctx v,
-    x ∈ l ->
-    (subst_local top x fv_u u ⦿ l) (ctx, v) = tvar v.
-Proof.
-  intros.
-  change (subst_local top x fv_u u (l ++ ctx, v) = tvar v).
-  unfold subst_local.
-  remember (SmartAtom.name_inb x (l ++ ctx)).
-  destruct b.
-  + reflexivity.
-  + false.
-    symmetry in Heqb.
-    rewrite SmartAtom.name_inb_iff_false in Heqb.
-    rewrite element_of_list_app in Heqb.
-    intuition.
-Qed.
-*)
-
-
-Lemma rename_binder_kill: forall top x fv_u l ctx v,
-    x ∈ l ->
-    (rename_binder_local top x fv_u ⦿ l) (ctx, v) = v.
-Proof.
-  intros.
-  change (rename_binder_local top x fv_u (l ++ ctx, v) = v).
-  unfold rename_binder_local.
-  rewrite ctx_to_history_app.
-Abort.
-
-Section proof_lemmas.
-
-  Context
-    (conflicts: list name)
-      (fv_u : list name)
-      (x: name) (u: term name name).
-
-  Implicit Types (ctx: list name) (v: name).
-
-  Lemma test:
-    ctx_to_history conflicts x fv_u [x] = [x].
-  Proof.
-    intros. cbn. destruct_eq_args x x.
-  Qed.
-
-  Lemma rename_binder_kill_corrected: forall ctx v,
-    (rename_binder_local conflicts x fv_u ⦿ [x]) (ctx, v) = v.
-  Proof.
-    intros.
-    change (rename_binder_local conflicts x fv_u ([x] ++ ctx, v) = v).
-    unfold rename_binder_local.
-    rewrite ctx_to_history_app.
-    generalize (fold_with_history
-                  (rename_binder_local_history conflicts x fv_u ⦿ fold_with_history
-                     (rename_binder_local_history conflicts x fv_u) [x])
-                  ctx).
-    intro l.
-    rewrite test.
-    unfo
-    Search rename_binder_local_history.
-    unfold rename_binder_local.
-    rewrite ctx_to_history_app.
-  Abort.
-
-
-Lemma kill:
-  forall (top fv_u: list name) (any: list name) (x: name) (t u: term name name),
-    x ∈ any ->
-    substitute (T := term) (G := fun A => A)
-      (rename_binder_local top x fv_u ⦿ any)
-      (subst_local top x fv_u u ⦿ any) t = t.
-Proof.
-  intros.
-  change t with (id t) at 2.
-  rewrite <- (kdtmp_substitute1 (T := term) (B := name) (A := name)).
-  fequal.
-  - ext (ctx, v).
-    try now apply rename_binder_kill.
-    admit.
-  - ext (ctx, v).
-Abort.
-
-
-Lemma substSmart_equiv:
-  forall (top: list name) (x: name) (u: term name name),
-    subst_top top x (FV term u) u =
-      substF top x u.
-Proof.
-  intros.
-  (* unfold subst_top. ext t. *)
-  intros. ext t. generalize dependent top. induction t; intros top.
-  - rewrite subst_top_rw1.
-    rewrite substF_rw1.
-    reflexivity.
-  - rewrite subst_top_rw2.
-    rewrite substF_rw2.
-    (* Is the binder the variable being substituted? *)
-    destruct_eq_args b x.
-    + (* Yes, it is. The RHS cuts off immediately. *)
-      (* We must show the LHS localized fns. are effectively the identity *)
-      fequal.
-      { unfold rename_binder_local.
-        rewrite ctx_to_history_nil.
-        rewrite rename_binder_local_history_rw1; auto.
-      }
-      { apply kill.
-        now simpl_list. }
-    + (* No, it's not *)
-      rewrite FV_fvL.
-      (* Is b of of the variables in fvL u and therefore needs to be renamed? *)
-      remember ((SmartAtom.name_inb b (fvL u))) as rem.
-      destruct rem.
-      * (* Yes, it is. Rename it. *)
-        fequal.
-        { unfold rename_binder_local.
-          assert (~ x ∈ nil) by easy.
-          rewrite <- inb_iff in H.
-          rewrite H.
-          destruct_eq_args x b.
-          rewrite <- Heqrem.
-          rewrite ctx_to_history_nil.
-          unfold rename_binder_local_history.
-          destruct_eq_args x b.
-          rewrite <- Heqrem.
-          rewrite List.app_nil_l.
-          reflexivity. }
-        {
-          admit.
-        }
-      * (* No, it's not. Don't rename it. *)
-        rewrite x1.
-        2:{ rewrite <- inb_iff. easy. }
-        rewrite <- IHt.
-        unfold subst_top.
-        fequal.
-        fequal.
-        { rewrite FV_fvL.
-          rewrite rename_binder_local_preincr; auto.
-          rewrite <- SmartAtom.name_inb_iff_false. easy.
-        }
-        {
-          rewrite subst_binder_preincr; auto.
-        }
-  - rewrite subst_top_rw3.
-    rewrite substF_rw3.
-    rewrite IHt1.
-    rewrite IHt2.
-    reflexivity.
-Admitted.
-
-
-
-Corollary substSmart_equiv_truly:
-  forall (x: name) (u: term name name) t,
-    substSmart x u t =
-      Raw.subst x u t.
-Proof.
-  intros.
-  unfold substSmart.
-  unfold Raw.subst.
-  rewrite FV_fvL.
-  rewrite FV_fvL.
-  apply substSmart_equiv.
-Qed.
-
-
-
-
-
-
-
-
-
-
-
-
-
-
-
-
-
-
-
-
-
-
-
-
-
-
-
-  (*
-  Lemma subst_conflicts_rw2: forall (top: list name) (b: name) (t: term name name),
-      subst_conflicts term top x u (lam b t) =
-        lam (rename_binder_local top ([], b))
-          (DecoratedTraversableMonadPoly.substitute (G := fun A => A)
-             (rename_binder_local top ⦿ [b])
-             (subst_local top x u ⦿ [b]) t).
-  Proof.
-    intros.
-    unfold subst.
-    unfold subst_conflicts.
-    unfold DecoratedTraversableMonadPoly.substitute.
-    unfold Binddt_Categorical.
-    unfold compose at 1 2 3 4.
-    rewrite dec_term_rw2.
-    rewrite map2_term_rw2.
-    rewrite dist2_unit.
-    unfold id.
-    unfold_ops @Map_I.
-    rewrite join_term_rw2.
-    fequal.
-    change (fun x : term name (term name name) => x) with
-      (@id (term name (term name name))).
-    change (?f ∘ id) with f.
-    compose near ([b], decp t) on left.
-    compose near (decp t) on left.
-    rewrite (map2_shift2_preincr
-               (g := (rename_binder_local top))
-               (f := (subst_local top x u))
-               (w := [b])).
-
-    reflexivity.
-  Qed.
-  *)
