Tealeaves/Backends/Named/NamedTraditionalV1.v
@@ -1,0 +1,361 @@
+
+
+
+
+
+
+
+
+
+
+
+
+
+
+
+
+
+
+
+
+
+
+
+
+
+
+
+
+
+
+
+    (* Given a substitution of x by u, encode the logic of what happens at <<current>> if <<history>> is the set of names
+       given to the binders so far *)
+    Definition rename_binder_local_history:
+      list name * name -> name :=
+      fun '(history, b) =>
+        if x == b
+        then b
+        else if SmartAtom.name_inb b (fv_u)
+             then fresh (conflicts ++ history ++ [b])
+             else if SmartAtom.name_inb b (conflicts ++ history)
+                  then fresh (conflicts ++ history ++ [b])
+                  else b.
+
+    Definition ctx_to_history: list name -> list name :=
+      fold_with_history rename_binder_local_history.
+
+    Lemma rename_binder_local_history_rw1 {hist b}:
+      b = x ->
+      rename_binder_local_history (hist, b) = b.
+    Proof.
+      intros.
+      unfold rename_binder_local_history.
+      destruct_eq_args x b.
+    Qed.
+
+    Lemma rename_binder_local_history_rw2 {hist b}:
+      b <> x ->
+      (b ∈ fv_u) ->
+      rename_binder_local_history (hist, b) = fresh (conflicts ++ hist ++ [b]).
+    Proof.
+      introv BneqX BinFVu.
+      unfold rename_binder_local_history.
+      destruct_eq_args x b.
+      rewrite <- SmartAtom.name_inb_iff in BinFVu.
+      rewrite BinFVu.
+      reflexivity.
+    Qed.
+
+    Lemma rename_binder_local_history_rw2' {b}:
+      b <> x ->
+      b ∈ fv_u ->
+      rename_binder_local_history (nil, b) = fresh (conflicts ++ [b]).
+    Proof.
+      intros.
+      rewrite rename_binder_local_history_rw2; auto.
+    Qed.
+
+
+    Lemma rename_binder_local_history_rw3 {hist b}:
+      b <> x ->
+      ~ (b ∈ fv_u) ->
+      (b ∈ (conflicts ++ hist)) ->
+      rename_binder_local_history (hist, b) = fresh (conflicts ++ hist ++ [b]).
+    Proof.
+      introv BneqX BinFVu BninHist.
+      unfold rename_binder_local_history.
+      destruct_eq_args x b.
+      rewrite <- SmartAtom.name_inb_iff_false in BinFVu.
+      rewrite BinFVu.
+      step_set_test.
+      reflexivity.
+    Qed.
+
+
+    Lemma rename_binder_local_history_rw4 {hist b}:
+      b <> x ->
+      ~ (b ∈ fv_u) ->
+      ~ (b ∈ (conflicts ++ hist)) ->
+      rename_binder_local_history (hist, b) = b.
+    Proof.
+      introv BneqX BinFVu BninHist.
+      unfold rename_binder_local_history.
+      destruct_eq_args x b.
+      rewrite <- SmartAtom.name_inb_iff_false in BinFVu.
+      rewrite BinFVu.
+      step_set_test.
+      reflexivity.
+    Qed.
+
+
+    Lemma ctx_to_history_nil: ctx_to_history [] = [].
+    Proof.
+      intros.
+      reflexivity.
+    Qed.
+
+    Lemma ctx_to_history_cons1 {nm l}:
+      x = nm ->
+      ctx_to_history (nm :: l) =
+        nm :: fold_with_history (rename_binder_local_history ⦿ [nm]) l.
+    Proof.
+      intros.
+      unfold ctx_to_history.
+      rewrite fold_with_history_cons.
+      rewrite rename_binder_local_history_rw1; auto.
+    Qed.
+
+
+    Lemma ctx_to_history_cons_cons2 {nm l}:
+      x <> nm ->
+      (nm ∈ fv_u) ->
+      ctx_to_history (nm :: l) =
+        fresh (conflicts ++ [nm]) :: fold_with_history (rename_binder_local_history ⦿ [fresh (conflicts ++ [nm])]) l.
+    Proof.
+      intros.
+      unfold ctx_to_history.
+      rewrite fold_with_history_cons.
+      rewrite rename_binder_local_history_rw2'; auto.
+    Qed.
+
+    Lemma ctx_to_history_cons_rw3 {nm l}:
+      x <> nm ->
+      ~ (nm ∈ fv_u) ->
+      nm ∈ (conflicts) ->
+      ctx_to_history (nm :: l) =
+        fresh (conflicts ++ [nm]) :: fold_with_history (rename_binder_local_history ⦿ [fresh (conflicts ++ [nm])]) l.
+    Proof.
+      intros.
+      unfold ctx_to_history.
+      rewrite fold_with_history_cons.
+      rewrite rename_binder_local_history_rw3; auto.
+      rewrite List.app_nil_r.
+      assumption.
+    Qed.
+
+    Lemma ctx_to_history_cons_rw4 {nm l}:
+      x <> nm ->
+      ~ (nm ∈ fv_u) ->
+      ~ nm ∈ (conflicts) ->
+      ctx_to_history (nm :: l) =
+        nm :: fold_with_history (rename_binder_local_history ⦿ [nm]) l.
+    Proof.
+      intros.
+      unfold ctx_to_history.
+      rewrite fold_with_history_cons.
+      rewrite rename_binder_local_history_rw4; auto.
+      rewrite List.app_nil_r.
+      assumption.
+    Qed.
+
+    Lemma ctx_to_history_app: forall l1 l2,
+        ctx_to_history (l1 ++ l2) =
+          ctx_to_history l1 ++
+            (fold_with_history (rename_binder_local_history ⦿ fold_with_history rename_binder_local_history l1) l2).
+    Proof.
+      intros.
+      unfold ctx_to_history.
+      rewrite fold_with_history_app.
+      reflexivity.
+    Qed.
+
+
+    (*
+
+    (* Name a binder to something else during substitution *)
+    Definition rename_binder_local:
+      list name * name -> name :=
+      fun '(ctx, b) =>
+        if SmartAtom.name_inb x ctx (* Halt substitution early, we didn't recurse where x appears in ctx *)
+        then b
+        else if x == b (* Else check if halt now *)
+             then b (* This binder is the name of the free variable we're substituting, halt and leave binder alone *)
+             else if SmartAtom.name_inb b fv_u (* Else check if need to rename *)
+                  then (rename_binder_local_history (ctx_to_history ctx, b))
+                  else b.
+
+    (* This binder is under an abstraction of the substituted variable, do nothing (subst halted earlier) *)
+    Lemma rename_binder_local_rw1: forall ctx b,
+        x ∈ ctx ->
+        rename_binder_local (ctx, b) = b.
+    Proof.
+      intros.
+      unfold rename_binder_local.
+      step_set_test.
+      reflexivity.
+    Qed.
+
+    (* This binder is equal to the variable begin substituted (subst is halting now) *)
+    Lemma rename_binder_local_rw2: forall ctx b,
+        ~ (x ∈ ctx) ->
+        x = b ->
+        rename_binder_local (ctx, b) = b.
+    Proof.
+      intros.
+      unfold rename_binder_local.
+      destruct_eq_args x b.
+      now step_set_test.
+    Qed.
+
+    (* This binder conflicts with the free variables of u, rename after computing its history from its context *)
+    Lemma rename_binder_local_rw3: forall ctx b,
+        ~ (x ∈ ctx) ->
+        x <> b ->
+        b ∈ fv_u ->
+        rename_binder_local (ctx, b) = (rename_binder_local_history (ctx_to_history ctx, b)).
+    Proof.
+      intros.
+      unfold rename_binder_local.
+      step_set_test.
+      destruct_eq_args x b.
+      step_set_test.
+      reflexivity.
+    Qed.
+
+    (* This is a bound variable that doesn't cause any conflicts, do nothing *)
+    Lemma rename_binder_local_rw4: forall ctx b,
+        ~ (x ∈ ctx) ->
+        x <> b ->
+        ~ (b ∈ fv_u) ->
+        rename_binder_local (ctx, b) = b.
+    Proof.
+      intros.
+      subst.
+      unfold rename_binder_local.
+      destruct (SmartAtom.name_inb x ctx); auto.
+      destruct_eq_args x b.
+      step_set_test.
+      reflexivity.
+    Qed.
+
+    Corollary rename_binder_local_rw5: forall ctx b,
+        ~ (b ∈ fv_u) ->
+        rename_binder_local (ctx, b) = b.
+    Proof.
+      intros.
+      unfold rename_binder_local.
+      destruct (SmartAtom.name_inb x ctx).
+      - reflexivity.
+      - destruct_eq_args x b.
+        step_set_test.
+        reflexivity.
+    Qed.
+
+    Lemma rename_binder_local_spec:
+      forall '(ctx, b),
+        rename_binder_local (ctx, b) = rename_binder_local_history (ctx_to_history ctx, b).
+    Proof.
+      intros [ctx b].
+      destruct (destruct_in x ctx).
+      rewrite rename_binder_local_rw1.
+      rewrite rename_binder_local_history_rw1.
+
+      step_set_test.
+      rewrite rename_binder_local_history_rw2.
+
+     *)
+
+ Definition rename_binder_local:
+      list name * name -> name :=
+   fun '(ctx, b) =>
+     rename_binder_local_history (ctx_to_history ctx, b).
+
+ Definition subst_local:
+   list name * name -> T name name :=
+   fun '(ctx, v) =>
+     if SmartAtom.name_inb x ctx (* Halt substitution early *)
+     then ret (T := T name) v
+     else
+       match (get_binding ctx v) with
+       | Unbound _ =>
+           if v == x
+           then u
+           else ret (T := T name) v
+       | Bound prefix _ _ =>
+           ret (T := T name) (rename_binder_local (prefix, v))
+       end.
+
+
+ (* This variable is under an abstraction of the substituted variable, do nothing (subst halted earlier) *)
+ Lemma subst_local_rw1: forall ctx v,
+     x ∈ ctx ->
+     subst_local (ctx, v) = ret v.
+ Proof.
+   intros.
+   unfold subst_local.
+   step_set_test.
+   reflexivity.
+ Qed.
+
+ (* This variable is equal to the variable begin substituted, replace it *)
+ Lemma subst_local_rw2: forall ctx v,
+     ~ (x ∈ ctx) ->
+     x = v ->
+     subst_local (ctx, v) = u.
+ Proof.
+   intros.
+   unfold subst_local.
+   destruct_eq_args x v.
+   step_set_test.
+   rewrite get_binding1; auto.
+ Qed.
+
+ Lemma hmmm:forall ctx v,
+     ~ v ∈ ctx ->
+     v = (rename_binder_local_history (ctx_to_history ctx, v)).
+ Proof.
+   intros.
+ Abort.
+
+
+ (* This is a bound variable that  conflicts with the free variables of u,
+       rename it to match its binder *)
+ Lemma subst_local_rw3: forall pre post ctx v,
+     ~ (x ∈ ctx) ->
+     x <> v ->
+     get_binding ctx v = Bound pre v post ->
+     subst_local (ctx, v) = ret (rename_binder_local_history (ctx_to_history pre, v)).
+ Proof.
+   intros.
+   unfold subst_local.
+   step_set_test.
+   rewrite H3.
+   unfold rename_binder_local.
+   reflexivity.
+ Qed.
+
+ Definition subst_top
+   (t: T name name): T name name :=
+   substitute (G := fun A => A) (U := T)
+     rename_binder_local
+     subst_local t.
+
+  End rename_local.
+
+  Definition subst
+    (x: name) (u: T name name)
+    (t: T name name): T name name :=
+    subst_top (FV T t ++ FV T u) x (FV T u) u t.
+
+End alt.
