Tealeaves/CompositionDemo.v
@@ -1,0 +1,120 @@
+From Tealeaves Require Import Tactics.Prelude.
+
+Open Scope tealeaves_scope.
+
+Set Printing Notations.
+
+Notation "(- ◻ g )" := (precompose g) (only parsing).
+Notation "( f ◻ -)" := (compose f) (only parsing).
+
+
+Context (A B C X Y Z Q R S: Type).
+Context (f: A -> B) (g: B -> C).
+
+Check g ∘ f.
+
+
+
+Check @compose A B C: (B -> C) -> (A -> B) -> A -> C.
+Check (@compose X (A -> B) (A -> C)) ∘ (@compose A B C): (B -> C) -> (X -> A -> B) -> X -> A -> C.
+Check (@compose X (A -> B) (A -> C)) ∘ (@compose A B C): (B -> C) -> (X -> A -> B) -> X -> A -> C.
+
+Check
+  (@compose A B C g): (A -> B) -> A -> C.
+
+Check
+  (@compose X (B -> C) ((A -> B) -> A -> C))
+    (@compose A B C): (X -> B -> C) -> X -> (A -> B) -> A -> C.
+
+Check
+  (@compose X (A -> B) (A -> C) (@compose A B C g)): (X -> A -> B) -> X -> A -> C.
+
+
+Context
+  (C1: A -> B)
+  (C2: A -> A -> B)
+  (C3: A -> A -> A -> B).
+
+Unset Printing Implicit.
+Unset Printing Notations.
+
+Check C1: A -> B.
+Check g ∘ C1: A -> C.
+
+Check C2: A -> A -> B.
+Check (@compose A B C g) ∘ C2: A -> A -> C.
+
+Check C3: A -> A -> A -> B.
+Check (@compose A (A -> B) (A -> C) (@compose A B C g) ∘ C3: A -> A -> A -> C).
+
+
+Section experiments1.
+
+  Context
+    (A': Type)
+      (f1: A' -> A)
+      (f2: A' -> A)
+      (f3: A' -> A).
+
+  Set Printing Notations.
+
+  Goal (fun a => C1 (f1 a)) = (precompose f1 C1).
+    reflexivity.
+  Qed.
+
+  Goal (fun a b => C2 (f1 a) (f2 b)) =
+         (((- ◻ f2) ◻ -) ◻ -) (- ◻ f1) C2.
+    reflexivity.
+  Qed.
+
+  Goal (fun a b => C2 (f1 a) (f2 b)) =
+         (((- ◻ f2) ◻ -) ∘ (- ◻ f1)) C2.
+    reflexivity.
+  Qed.
+
+  Goal (fun a b => C2 (f1 a) (f2 b)) =
+         (compose ((- ◻ f2) ◻ -) (- ◻ f1)) C2.
+    reflexivity.
+  Qed.
+
+End experiments1.
+
+
+
+Section experiments2.
+
+  Context
+    (A A' B': Type)
+      (C: A -> B) (g: A' -> A) (f: B -> B').
+
+  Goal (f ∘ C ∘ g) =
+         (compose f ∘ precompose g) C.
+    reflexivity.
+  Qed.
+
+  Goal (f ∘ C ∘ g) =
+         ((f ◻ -) ∘ (- ◻ g)) C.
+    reflexivity.
+  Qed.
+
+  Goal (f ∘ (fun x => C (g x))) =
+         (compose f ∘ precompose g) C.
+    reflexivity.
+  Qed.
+
+  Goal (fun a b => C2 (f1 a) (f2 b)) =
+         (((- ◻ f2) ◻ -) ◻ -) (- ◻ f1) C2.
+    reflexivity.
+  Qed.
+
+  Goal (fun a b => C2 (f1 a) (f2 b)) =
+         (((- ◻ f2) ◻ -) ∘ (- ◻ f1)) C2.
+    reflexivity.
+  Qed.
+
+  Goal (fun a b => C2 (f1 a) (f2 b)) =
+         (compose ((- ◻ f2) ◻ -) (- ◻ f1)) C2.
+    reflexivity.
+  Qed.
+
+End experiments1.
